

Wald test statistic for Normal distribution

The general form of W statistic is

$$W = \frac{\hat{\theta} - \theta}{\sqrt{\text{var}(\hat{\theta})}}$$

For a given sample, we genially plug in the estimated $\text{var}(\hat{\theta})$ to the denominator, i.e.,

$$W = \frac{\hat{\theta} - \theta}{\sqrt{\widehat{\text{var}}(\hat{\theta})}}$$

In the following hypothesis test, $X \sim N(\mu, \sigma^2)$, where μ and σ^2 are unknown.

$$H_0: \mu = \mu_0$$

$$H_1: \mu \neq \mu_0$$

The Maximum likelihood estimator of μ is

$$\hat{\mu} = \bar{X}_n$$

The sample variance of $\hat{\mu}$ is

$$\begin{aligned}\widehat{\text{var}}(\hat{\mu}) &= \widehat{\text{var}}(\bar{X}_n) = \widehat{\text{var}}\left(\frac{1}{n} \sum_{i=1}^n X_i\right) = \frac{1}{n^2} \widehat{\text{var}}\left(\sum_{i=1}^n X_i\right) = \frac{n}{n^2} \widehat{\text{var}}(X_i) \\ &= \frac{\hat{\sigma}^2}{n}\end{aligned}$$

Next find an estimator for $\hat{\sigma}^2$.

Consider

$$\hat{\sigma}^2 = s_n^2 = \frac{1}{n-1} \sum_{i=1}^n (X_i - \bar{X}_n)^2$$

It can be proved (below) that s_n^2 is an unbiased estimator of σ^2 , i.e., $E(s_n^2) = \sigma^2$.

Proof

$$\begin{aligned}E(s_n^2) &= E\left[\frac{1}{n-1} \sum_{i=1}^n (X_i - \bar{X}_n)^2\right] = \frac{1}{n-1} E\left[\sum_{i=1}^n X_i^2 + n(\bar{X}_n)^2 - 2 \sum_{i=1}^n X_i \bar{X}_n\right] \\ &= \frac{1}{n-1} E\left[\sum_{i=1}^n X_i^2 - n(\bar{X}_n)^2\right] = \frac{1}{n-1} [nE(X_i^2) - nE(\bar{X}_n^2)] \\ &= \frac{n}{n-1} [E(X_i^2) - E(\bar{X}_n^2)] \\ &= \frac{n}{n-1} ([E(X_i)^2 + \text{Var}(X_i)] - [E(\bar{X}_n)^2 + \text{Var}(\bar{X}_n)]) \\ &= \frac{n}{n-1} \left([\mu^2 + \sigma^2] - \left[\mu^2 + \frac{1}{n} \text{Var}(X_i)\right]\right) = \frac{n}{n-1} \times \left(\frac{n-1}{n} \sigma^2\right) = \sigma^2\end{aligned}$$

QED

Plugging $s_n^2 = \frac{1}{n-1} \sum_{i=1}^n (X_i - \bar{X}_n)^2$ into $\widehat{var}(\hat{\mu})$ yields

$$\widehat{var}(\hat{\mu}) = \frac{\hat{\sigma}^2}{n} = \frac{s_n^2}{n}$$

So, the W statistic is

$$\frac{\hat{\mu} - \mu}{\sqrt{\widehat{var}(\hat{\mu})}} = \frac{\hat{\mu} - \mu}{\sqrt{\frac{s_n^2}{n}}} = \frac{\sqrt{n}(\bar{X}_n - \mu_0)}{\sqrt{s_n^2}} = \frac{\sqrt{n}(\bar{X}_n - \mu_0)}{\sqrt{\frac{1}{n-1} \sum_{i=1}^n (X_i - \bar{X}_n)^2}}$$